Finalize theoretic background for PreStar algorithm

Lemke/Algorithm.thy
@@ -1,167 +1,319 @@
 section\<open>Computing $pre^*(L)$\<close>
 
 theory Algorithm
-  imports Definition FiniteAutomaton
+  imports Definition FiniteAutomaton "HOL-Library.While_Combinator"
 begin \<comment>\<open>begin-theory Algorithm\<close>
 
 context CFG
 begin \<comment>\<open>begin-context CFG\<close>
 
-fun prestar_nfa_t :: "('s \<times> ('n, 't) sym \<times> 's) set \<Rightarrow> nat \<Rightarrow> ('s \<times> ('n, 't) sym \<times> 's) set" where
-  "prestar_nfa_t T (Suc n) = (
-    let T' = prestar_nfa_t T n in
-    T' \<union> { (q, Nt A, q') | q q' A. \<exists>\<beta>. (A, \<beta>) \<in> P \<and> q' \<in> steps T' \<beta> q }
-  )" |
-  "prestar_nfa_t T 0 = T"
 
-lemma prestar_nfa_t_converges:
-  fixes T :: "('s \<times> ('n, 't) sym \<times> 's) set"
-  assumes "finite (UNIV::'s set)" \<comment>\<open>Only works if states are finite.\<close>
-  shows "\<exists>n. \<forall>n'. prestar_nfa_t T n' = prestar_nfa_t T n"
-  sorry
+
+definition prestar_step :: "('s \<times> ('n, 't) sym \<times> 's) set \<Rightarrow> ('s \<times> ('n, 't) sym \<times> 's) set" where
+  "prestar_step T \<equiv> { (q, Nt A, q') | q q' A. \<exists>\<beta>. (A, \<beta>) \<in> P \<and> q' \<in> steps T \<beta> q }"
+
+definition prestar_while :: "('s \<times> ('n, 't) sym \<times> 's) set \<Rightarrow> ('s \<times> ('n, 't) sym \<times> 's) set option" where
+  "prestar_while \<equiv> while_option (\<lambda>T. T \<union> prestar_step T \<noteq> T) (\<lambda>T. T \<union> prestar_step T)"
+
+
+
+lemma nfa_mono':
+  assumes "T\<^sub>1 \<subseteq> T\<^sub>2" and "q\<^sub>1 \<subseteq> q\<^sub>2"
+  shows "steps' T\<^sub>1 w q\<^sub>1 \<subseteq> steps' T\<^sub>2 w q\<^sub>2"
+proof (insert assms(2); induction w arbitrary: q\<^sub>1 q\<^sub>2)
+  case Nil thus ?case by simp
+next
+  case (Cons w ws)
+  have "step' T\<^sub>1 w q\<^sub>1 \<subseteq> step' T\<^sub>2 w q\<^sub>2"
+    using assms(1) Cons(2) by auto
+  then have "steps' T\<^sub>1 ws (step' T\<^sub>1 w q\<^sub>1) \<subseteq> steps' T\<^sub>1 ws (step' T\<^sub>2 w q\<^sub>2)"
+    by (rule steps'_mono)
+  then have "steps' T\<^sub>1 ws (step' T\<^sub>1 w q\<^sub>1) \<subseteq> steps' T\<^sub>2 ws (step' T\<^sub>2 w q\<^sub>2)"
+    using Cons(1) by blast
+  then show ?case
+    by simp
+qed
+
+lemma nfa_mono: "T\<^sub>1 \<subseteq> T\<^sub>2 \<Longrightarrow> steps T\<^sub>1 w q \<subseteq> steps T\<^sub>2 w q"
+  using nfa_mono'[of T\<^sub>1 T\<^sub>2 "{q}" "{q}" w] by simp
+
+lemma nfa_lang_mono: "T\<^sub>1 \<subseteq> T\<^sub>2 \<Longrightarrow> lang' T\<^sub>1 s f \<subseteq> lang' T\<^sub>2 s f"
+  unfolding lang'_def accepts_def using nfa_mono[of T\<^sub>1 T\<^sub>2] by fast
+
+
+
+lemma prestar_while_mono:
+  assumes "prestar_while T\<^sub>0 = Some T'"
+  shows "T\<^sub>0 \<subseteq> T'"
+  unfolding prestar_while_def
+proof (rule while_option_rule[where P = "\<lambda>T. T\<^sub>0 \<subseteq> T", OF _ assms[unfolded prestar_while_def]])
+  show "T\<^sub>0 \<subseteq> T\<^sub>0"
+    by blast
+next
+  fix T
+  assume "T\<^sub>0 \<subseteq> T" and "T \<union> prestar_step T \<noteq> T"
+  then show "T\<^sub>0 \<subseteq> T \<union> prestar_step T"
+    by blast
+qed
+
+lemma prestar_step_mono: "mono (\<lambda>T. T \<union> prestar_step T)"
+proof -
+  have "\<And>A B. A \<subseteq> B \<Longrightarrow> prestar_step A \<subseteq> prestar_step B"
+  proof (standard)
+    fix A :: "('s \<times> ('n, 't) sym \<times> 's) set" and B and w
+    assume assm1: "A \<subseteq> B" and assm2: "w \<in> prestar_step A"
+    obtain q q' \<alpha> \<beta> where [simp]: "w = (q, Nt \<alpha>, q')" and [simp]: "(\<alpha>, \<beta>) \<in> P" and "q' \<in> steps A \<beta> q"
+      using assm2 prestar_step_def by (smt (verit, best) mem_Collect_eq)
+    then have "q' \<in> steps B \<beta> q"
+      using nfa_mono[of A B] assm1 by blast
+    then show "w \<in> prestar_step B"
+      unfolding prestar_step_def by force
+  qed
+  then show ?thesis
+    by (intro monoI, blast)
+qed
+
+
+
+lemma finite_univ_tuple[intro]:
+  assumes "finite (UNIV::'a set)" and "finite (UNIV::'b set)"
+  shows "finite (UNIV::('a \<times> 'b) set)"
+  by (simp add: assms(1,2) finite_Prod_UNIV)
+
+lemma prestar_while_terminates:
+  fixes T\<^sub>0 :: "('s \<times> ('n, 't) sym \<times> 's) set"
+  assumes "finite (UNIV::'s set)"
+  shows "\<exists>T. prestar_while T\<^sub>0 = Some T"
+proof -
+  have "finite ({ Nt x | x::'n. True } \<union> { Tm x | x::'t. True })"
+  proof (rule finite_UnI)
+    have "inj_on (\<lambda>x. (Nt x::('n, 't) sym)) (UNIV::'n set)"
+      by (rule injI, simp)
+    moreover have "finite (UNIV::'n set)"
+      using CFG_axioms by (simp add: CFG_def)
+    ultimately show "finite ({ Nt x | x. True }::('n, 't) sym set)"
+      using finite_image_iff by (simp add: full_SetCompr_eq)
+  next
+    have "inj_on (\<lambda>x. (Tm x::('n, 't) sym)) (UNIV::'t set)"
+      by (rule injI, simp)
+    moreover have "finite (UNIV::'t set)"
+      using CFG_axioms by (simp add: CFG_def)
+    ultimately show "finite ({ Tm x | x. True }::('n, 't) sym set)"
+      using finite_image_iff by (simp add: full_SetCompr_eq)
+  qed
+  then have "finite (UNIV::('n, 't) sym set)"
+    by (smt (verit, ccfv_threshold) UNIV_eq_I Un_def mem_Collect_eq sym.exhaust)
+  then have "finite (UNIV::('s \<times> ('n, 't) sym \<times> 's) set)"
+    using assms by blast
+  then have "finite (UNIV::(('s \<times> ('n, 't) sym \<times> 's) set) set)"
+    by (simp add: Finite_Set.finite_set)
+  moreover have "T\<^sub>0 \<le> T\<^sub>0 \<union> prestar_step T\<^sub>0"
+    by simp
+  ultimately show ?thesis
+    unfolding prestar_while_def
+    using prestar_step_mono by (intro while_option_finite_increasing_Some; simp_all)
+qed
+
+lemma prestar_while_fixpoint:
+  assumes "prestar_while T\<^sub>0 = Some T"
+  shows "T \<union> prestar_step T = T"
+proof -
+  have "\<not> (T \<union> prestar_step T \<noteq> T)"
+    by (insert assms[unfolded prestar_while_def], rule while_option_stop)
+  then have "T \<union> prestar_step T = T"
+    by simp
+  then show ?thesis .
+qed
+
+
+
+lemma prestar_saturated_step:
+  assumes "X\<^sub>1 \<Rightarrow> X\<^sub>2" and "q' \<in> steps T\<^sub>0 X\<^sub>2 q"
+  shows "q' \<in> steps (T\<^sub>0 \<union> prestar_step T\<^sub>0) X\<^sub>1 q"
+proof -
+  define T where [simp]: "T \<equiv> T\<^sub>0 \<union> prestar_step T\<^sub>0"
+  obtain \<alpha> w\<^sub>1 w\<^sub>2 \<beta> where X\<^sub>1_def: "X\<^sub>1 = \<alpha>@[Nt w\<^sub>1]@\<beta>" and X\<^sub>2_def: "X\<^sub>2 = \<alpha>@w\<^sub>2@\<beta>" and "(w\<^sub>1, w\<^sub>2) \<in> P"
+    by (metis (mono_tags, opaque_lifting) assms(1) prods_to_lts.cases step_relp_def transition_relation_def)
+  obtain s s' where "s \<in> steps T\<^sub>0 \<alpha> q" and "s' \<in> steps T\<^sub>0 w\<^sub>2 s" and "q' \<in> steps T\<^sub>0 \<beta> s'"
+    using steps_split3 assms(2) X\<^sub>2_def by fastforce
+  then have "(s, Nt w\<^sub>1, s') \<in> prestar_step T\<^sub>0"
+    unfolding prestar_step_def using \<open>(w\<^sub>1, w\<^sub>2) \<in> P\<close> by blast
+  then have "(s, Nt w\<^sub>1, s') \<in> T"
+    by simp
+  then have "s' \<in> steps T [Nt w\<^sub>1] s"
+    by simp
+  moreover have "s \<in> steps T \<alpha> q"
+    using \<open>s \<in> steps T\<^sub>0 \<alpha> q\<close> T_def nfa_mono[of T\<^sub>0 T] by blast
+  moreover have "q' \<in> steps T \<beta> s'"
+    using \<open>q' \<in> steps T\<^sub>0 \<beta> s'\<close> T_def nfa_mono[of T\<^sub>0 T] by blast
+  ultimately have "q' \<in> steps T (\<alpha>@[Nt w\<^sub>1]@\<beta>) q"
+    using steps_join3 by fast
+  then show ?thesis
+    using X\<^sub>1_def by simp
+qed
+
+lemma prestar_saturated:
+  assumes "X\<^sub>1 \<Rightarrow> X\<^sub>2" and "q' \<in> steps T X\<^sub>2 q"
+    and "prestar_while T\<^sub>0 = Some T"
+  shows "q' \<in> steps T X\<^sub>1 q"
+proof -
+  have "T \<union> prestar_step T = T"
+    using prestar_while_fixpoint assms(3) by blast
+  moreover have "q' \<in> steps (T \<union> prestar_step T) X\<^sub>1 q"
+    using assms prestar_saturated_step by fast
+  ultimately show ?thesis
+    by simp
+qed
+
+lemma prestar_saturated_lang:
+  assumes "prestar_while T\<^sub>0 = Some T"
+  shows "pre_star (lang' T\<^sub>0 s F) \<subseteq> lang' T s F"
+proof (standard)
+  fix w
+  assume "w \<in> pre_star (lang' T\<^sub>0 s F)"
+  then obtain w' where "w \<Rightarrow>\<^sup>* w'" and "w' \<in> lang' T\<^sub>0 s F"
+    unfolding pre_star_def by blast
+  then show "w \<in> lang' T s F"
+  proof (induction rule: converse_rtranclp_induct[where r="(\<Rightarrow>)"])
+    case base
+    moreover have "T\<^sub>0 \<subseteq> T"
+      by (simp add: assms prestar_while_mono)
+    ultimately show ?case
+      using nfa_lang_mono[of T\<^sub>0 T s F] by blast
+  next
+    case (step y z)
+    then have "z \<in> lang' T s F"
+      by simp
+    then obtain q\<^sub>f where "q\<^sub>f \<in> steps T z s" and "q\<^sub>f \<in> F"
+      unfolding lang'_def accepts_def by fastforce
+    then have "q\<^sub>f \<in> steps T y s" and "q\<^sub>f \<in> F"
+      using assms step(1) prestar_saturated[of y z q\<^sub>f T s] by simp+
+    then show ?case
+      unfolding lang'_def accepts_def by fastforce
+  qed
+qed
+
+
+
+lemma prestar_triple_trans[trans]:
+  assumes "A \<subseteq> pre_star B"
+    and "B \<subseteq> pre_star C"
+  shows "A \<subseteq> pre_star C"
+proof -
+  have "\<forall>w \<in> A. \<exists>w' \<in> B. w \<Rightarrow>\<^sup>* w'"
+    using assms(1) pre_star_def by blast
+  moreover have "\<forall>w \<in> B. \<exists>w' \<in> C. w \<Rightarrow>\<^sup>* w'"
+    using assms(2) pre_star_def by blast
+  ultimately have "\<forall>w \<in> A. \<exists>w' \<in> C. w \<Rightarrow>\<^sup>* w'"
+    using rtranclp_trans by fast
+  then show ?thesis
+    unfolding pre_star_def by blast
+qed
+
+lemma prestar_saturator: "lang' (T \<union> prestar_step T) s F \<subseteq> pre_star (lang' T s F)"
+proof (standard)
+  fix w
+  assume "w \<in> lang' (T \<union> prestar_step T) s F"
+  then show "w \<in> pre_star (lang' T s F)"
+  proof (induction w arbitrary: s)
+    case Nil
+    then have "[] \<in> lang' T s F"
+      by (simp add: lang'_def accepts_def)
+    moreover have "[] \<Rightarrow>\<^sup>* []"
+      by simp
+    ultimately show ?case
+      unfolding pre_star_def by blast
+  next
+    case (Cons w ws)
+    then have "[w]@ws \<in> lang' (T \<union> prestar_step T) s F"
+      by simp
+    then obtain s' where s'_step: "s' \<in> steps (T \<union> prestar_step T) [w] s"
+        and "ws \<in> lang' (T \<union> prestar_step T) s' F"
+      by (rule nfa_lang_split, simp)
+    then have "ws \<in> pre_star (lang' T s' F)"
+      by (simp add: Cons(1))
+    then obtain ws' where "ws \<Rightarrow>\<^sup>* ws'" and ws'_lang: "ws' \<in> lang' T s' F"
+      unfolding pre_star_def by blast
+
+    have "(s, w, s') \<in> T \<or> (s, w, s') \<in> prestar_step T"
+      using s'_step by simp
+    then show ?case
+    proof (standard)
+      assume "(s, w, s') \<in> T"
+      then have "s' \<in> step T w s"
+        by simp
+      then have "s' \<in> steps T [w] s"
+        by simp
+      moreover note \<open>ws' \<in> lang' T s' F\<close>
+      ultimately have "(w#ws') \<in> lang' T s F"
+        using nfa_lang_trans by fastforce
+      then show "(w#ws) \<in> pre_star (lang' T s F)"
+        unfolding pre_star_def using \<open>ws \<Rightarrow>\<^sup>* ws'\<close> derives_Cons derives_eq by blast
+    next
+      assume "(s, w, s') \<in> prestar_step T"
+      then obtain A \<beta> where "w = Nt A" and "(A, \<beta>) \<in> P" and "s' \<in> steps T \<beta> s"
+        unfolding prestar_step_def by blast
+      moreover note \<open>ws' \<in> lang' T s' F\<close>
+      ultimately have "(\<beta>@ws') \<in> lang' T s F"
+        using nfa_lang_trans by fastforce
+      moreover have "(w#ws) \<Rightarrow>\<^sup>* (\<beta>@ws')"
+        using \<open>w = Nt A\<close> \<open>(A, \<beta>) \<in> P\<close> \<open>ws \<Rightarrow>\<^sup>* ws'\<close>
+        by (meson derives_Cons_rule derives_eq derives_prepend)
+      ultimately show "(w#ws) \<in> pre_star (lang' T s F)"
+        unfolding pre_star_def by blast
+    qed
+  qed
+qed
+
+lemma prestar_saturator_lang:
+  assumes "prestar_while T\<^sub>0 = Some T"
+  shows "lang' T s F \<subseteq> pre_star (lang' T\<^sub>0 s F)"
+  unfolding prestar_while_def
+proof (rule while_option_rule[where P = "\<lambda>T. lang' T s F \<subseteq> pre_star (lang' T\<^sub>0 s F)", OF _ assms[unfolded prestar_while_def]])
+  show "lang' T\<^sub>0 s F \<subseteq> pre_star (lang' T\<^sub>0 s F)"
+    unfolding pre_star_def by blast
+next
+  fix T
+  assume "lang' T s F \<subseteq> pre_star (lang' T\<^sub>0 s F)"
+    and "T \<union> prestar_step T \<noteq> T"
+  moreover have "lang' (T \<union> prestar_step T) s F \<subseteq> pre_star (lang' T s F)"
+    by (rule prestar_saturator)
+  ultimately show "lang' (T \<union> prestar_step T) s F \<subseteq> pre_star (lang' T\<^sub>0 s F)"
+    using prestar_triple_trans by blast
+qed
+
+
+
+lemma prestar_while_lang:
+  assumes "prestar_while T\<^sub>0 = Some T"
+  shows "lang' T s F = pre_star (lang' T\<^sub>0 s F)"
+  using prestar_saturated_lang prestar_saturator_lang assms by fast
 
 definition prestar_nfa :: "('s, ('n, 't) sym) nfa \<Rightarrow> ('s, ('n, 't) sym) nfa" where
   "prestar_nfa M \<equiv> (
-    let n = THE n. \<forall>n'. prestar_nfa_t (transitions M) n' = prestar_nfa_t (transitions M) n in
-    M \<lparr> transitions := prestar_nfa_t (transitions M) n \<rparr>
+    case prestar_while (transitions M) of
+      Some t \<Rightarrow> M \<lparr> transitions := t \<rparr> |
+      None \<Rightarrow> undefined
   )"
 
-lemma nfa_transitions_mono:
-  assumes "transitions M\<^sub>1 \<subseteq> transitions M\<^sub>2"
-    and "start M\<^sub>1 = start M\<^sub>2"
-    and "finals M\<^sub>1 \<subseteq> finals M\<^sub>2"
-  shows "lang M\<^sub>1 \<subseteq> lang M\<^sub>2"
-  sorry
-
-lemma nfa_transitions_mono': "lang M \<subseteq> lang (M \<lparr> transitions := transitions M \<union> T \<rparr>)"
-proof -
-  define M' where "M' = M \<lparr> transitions := transitions M \<union> T \<rparr>"
-  moreover have "transitions M \<subseteq> transitions M'" and "start M = start M'" and "finals M \<subseteq> finals M'"
-    by (simp add: M'_def)+
-  ultimately show ?thesis
-    using nfa_transitions_mono by blast
-qed
-
-lemma prestar_nfa_mono:
-  fixes M :: "('s, ('n, 't) sym) nfa"
-  assumes "finite (UNIV::'s set)"
-  shows "lang M \<subseteq> lang (prestar_nfa M)"
-proof -
-  let ?M = "\<lambda>n. M \<lparr> transitions := prestar_nfa_t (transitions M) n \<rparr>"
-
-  define M' where "M' = prestar_nfa M"
-  moreover obtain n where n_def: "\<forall>n'. prestar_nfa_t (transitions M) n' = prestar_nfa_t (transitions M) n"
-    using assms prestar_nfa_t_converges by blast
-  ultimately have M'_trans: "M' = ?M n"
-    by (simp add: prestar_nfa_def)
-
-  have "lang M \<subseteq> lang (?M n)"
-  proof (induction "transitions M" n rule: prestar_nfa_t.induct)
-    case (1 n)
-    moreover have "lang (?M n) \<subseteq> lang (?M (Suc n))"
-      by (metis n_def order_refl)
-    ultimately show ?case by simp
-  next
-    case 2 thus ?case by simp
-  qed
-  then show ?thesis
-    using M'_def M'_trans by simp
-qed
-
-lemma prestar_nfa_saturated:
-  fixes M :: "('s, ('n, 't) sym) nfa"
-  assumes "finite (UNIV::'s set)"
-    and "(A, \<beta>) \<in> P" and "q' \<in> steps (transitions (prestar_nfa M)) \<beta> q"
-  shows "(q, Nt A, q') \<in> transitions (prestar_nfa M)"
-proof -
-  define M' where "M' = prestar_nfa M"
-  moreover obtain n where n_def: "\<forall>n'. prestar_nfa_t (transitions M) n' = prestar_nfa_t (transitions M) n"
-    using assms prestar_nfa_t_converges by blast
-  ultimately have M'_trans: "M' = M \<lparr> transitions := prestar_nfa_t (transitions M) n \<rparr>"
-    by (simp add: prestar_nfa_def)
-
-  have "\<And>n. q' \<in> steps (prestar_nfa_t (transitions M) n) \<beta> q \<Longrightarrow> (q, Nt A, q') \<in> prestar_nfa_t (transitions M) (Suc n)"
-    subgoal for n
-    proof (induction "transitions M" n rule: prestar_nfa_t.induct)
-      case (1 n)
-      then show ?case
-        using assms(2) by (metis n_def)
-    next
-      case 2
-      then show ?case
-        using assms(2) sorry
-    qed
-    done
-
-  show ?thesis sorry
-qed
-
-lemma prestar_nfa1:
-  fixes M :: "('s, ('n, 't) sym) nfa"
-  assumes "finite (UNIV::'s set)"
-  shows "pre_star (lang M) \<subseteq> lang (prestar_nfa M)"
-proof -
-  define M' where "M' = prestar_nfa M"
-  moreover obtain n where "\<forall>n'. prestar_nfa_t (transitions M) n' = prestar_nfa_t (transitions M) n"
-    using assms prestar_nfa_t_converges by blast
-  ultimately have M'_trans: "M' = M \<lparr> transitions := prestar_nfa_t (transitions M) n \<rparr>"
-    by (simp add: prestar_nfa_def)
-
-  have "\<And>\<alpha>. \<alpha> \<in> pre_star (lang M) \<Longrightarrow> \<alpha> \<in> lang (prestar_nfa M)"
-  proof -
-    fix \<alpha>
-    assume "\<alpha> \<in> pre_star (lang M)"
-    then obtain \<beta> where "\<alpha> \<Rightarrow>\<^sup>* \<beta>" and "\<beta> \<in> lang M"
-      unfolding pre_star_def by blast
-    then show "\<alpha> \<in> lang (prestar_nfa M)"
-    proof (induction rule: converse_rtranclp_induct[where r="(\<Rightarrow>)"])
-      case base
-      then show ?case
-        using assms prestar_nfa_mono by blast
-    next
-      case (step \<alpha> \<gamma>)
-
-      define T where [simp add]: "T = transitions (prestar_nfa M)"
-      define q\<^sub>0 where [simp add]: "q\<^sub>0 = start (prestar_nfa M)"
-
-      obtain \<alpha>\<^sub>1 \<alpha>\<^sub>2 \<alpha>\<^sub>3 A where "\<alpha> = \<alpha>\<^sub>1@[Nt A]@\<alpha>\<^sub>3" and "\<gamma> = \<alpha>\<^sub>1@\<alpha>\<^sub>2@\<alpha>\<^sub>3" and "(A, \<alpha>\<^sub>2) \<in> P"
-        using step(1) by (metis (mono_tags, opaque_lifting) prods_to_lts.simps step_relp_def transition_relation_def)
-
-      have "\<gamma> \<in> lang (prestar_nfa M)"
-        by (simp add: step)
-      then have "accepts (prestar_nfa M) (\<alpha>\<^sub>1@\<alpha>\<^sub>2@\<alpha>\<^sub>3)"
-        using \<open>\<gamma> = \<alpha>\<^sub>1@\<alpha>\<^sub>2@\<alpha>\<^sub>3\<close> lang_def by blast
-      then obtain q q' q\<^sub>f where step1: "q \<in> steps T \<alpha>\<^sub>1 q\<^sub>0" and step2: "q' \<in> steps T \<alpha>\<^sub>2 q"
-          and step3: "q\<^sub>f \<in> steps T \<alpha>\<^sub>3 q'" and [simp add]: "q\<^sub>f \<in> finals (prestar_nfa M)"
-        using accepts_split3[of "prestar_nfa M" \<alpha>\<^sub>1 \<alpha>\<^sub>2 \<alpha>\<^sub>3] by fastforce
-
-      have "(q, Nt A, q') \<in> T"
-        using prestar_nfa_saturated assms \<open>(A, \<alpha>\<^sub>2) \<in> P\<close> step2 by fastforce
-      then have "q' \<in> steps T [Nt A] q"
-        by simp
-      then have "q\<^sub>f \<in> steps T (\<alpha>\<^sub>1@[Nt A]@\<alpha>\<^sub>3) q\<^sub>0"
-        using step1 step3 steps_join3 by fast
-      then have "accepts (prestar_nfa M) (\<alpha>\<^sub>1@[Nt A]@\<alpha>\<^sub>3)"
-        by fastforce
-      then show ?case
-        unfolding lang_def \<open>\<alpha> = \<alpha>\<^sub>1@[Nt A]@\<alpha>\<^sub>3\<close> by simp
-    qed
-  qed
-  then show ?thesis
-    using M'_def M'_trans by blast
-qed
-
-lemma prestar_nfa2:
-  fixes M :: "('s, ('n, 't) sym) nfa"
-  assumes "finite (UNIV::'s set)"
-  shows "lang (prestar_nfa M) \<subseteq> pre_star (lang M)"
-  sorry
-
-theorem prestar_nfa:
+theorem prestar_nfa_lang:
   fixes M :: "('s, ('n, 't) sym) nfa"
   assumes "finite (UNIV::'s set)"
   shows "lang (prestar_nfa M) = pre_star (lang M)"
-  using assms prestar_nfa1 prestar_nfa2 by blast
+proof -
+  define T\<^sub>0 where [simp]: "T\<^sub>0 = transitions M"
+  define M' where [simp]: "M' = prestar_nfa M"
+  define T where [simp]: "T = transitions M'"
+
+  have "\<exists>T. prestar_while T\<^sub>0 = Some T"
+    using assms by (rule prestar_while_terminates)
+  then have "prestar_while T\<^sub>0 = Some T"
+    by (auto simp: prestar_nfa_def)
+  moreover have "start M = start M'" and "finals M = finals M'"
+    unfolding M'_def prestar_nfa_def using calculation by simp+
+  ultimately show ?thesis
+    by (simp add: prestar_while_lang)
+qed
 
 end \<comment>\<open>end-context CFG\<close>
 
